Logic/FirstOrder/Class/Class.lean
@@ -16,13 +16,6 @@ lemma hom_eq_id_of_eq_on_fvar_list (ω : Rew L μ n μ n) (hb : ∀ x, ω (#x) =
   · simpa using hb
   · intro x hx; simp [hf x hx]
 
-@[simp] lemma rewriteMap_fvEnumInv_fvEnum [DecidableEq ξ] [Inhabited ξ] (q : Semiformula L ξ n) :
-    (Rew.rewriteMap (q.fvEnumInv ∘ q.fvEnum)).hom q = q :=
-  hom_eq_id_of_eq_on_fvar_list _ (by simp) (fun x hx ↦ by simp [Semiformula.fvEnumInv_fvEnum hx])
-
-lemma rewrite_eq_rewriteMap (f : ξ₁ → ξ₂) :
-    (Rew.rewrite fun x ↦ &(f x) : Rew L ξ₁ n ξ₂ n) = Rew.rewriteMap f := rfl
-
 end Rew
 
 variable {L : Language} {ξ : Type*} [DecidableEq ξ]
@@ -82,6 +75,12 @@ lemma ex {p₁ p₂ : Semiformula L ξ (n + 1)} (hp : p₁ ↔[T] p₂) : (∃' 
   apply exists_congr; intro a
   exact hp M x hT ε (a :> e)
 
+lemma ball {p₁ p₂ q₁ q₂ : Semiformula L ξ (n + 1)} (hp : p₁ ↔[T] p₂) (hq : q₁ ↔[T] q₂) : (∀[p₁] q₁) ↔[T] (∀[p₂] q₂) :=
+  all (imp hp hq)
+
+lemma bex {p₁ p₂ q₁ q₂ : Semiformula L ξ (n + 1)} (hp : p₁ ↔[T] p₂) (hq : q₁ ↔[T] q₂) : (∃[p₁] q₁) ↔[T] (∃[p₂] q₂) :=
+  ex (and hp hq)
+
 lemma all_and_all (p q : Semiformula L ξ (n + 1)) :
     ((∀' p) ⋏ (∀' q)) ↔[T] (∀' ∀' ((Rew.substs (#1 :> (#·.succ.succ))).hom p ⋏ (Rew.substs (#0 :> (#·.succ.succ))).hom q)) := by
   simp [Equivalent, consequence_iff, models_iff, eval_substs, Matrix.comp_vecCons']
@@ -135,7 +134,7 @@ def RewClosure (C : Semiformula L ξ n → Prop) : Semiformula L ξ n → Prop :
 
 def EqvClosure (T : Theory L) (C : Semiformula L ξ n → Prop) : Semiformula L ξ n → Prop := fun p ↦ ∃ p₀, C p₀ ∧ p₀ ↔[T] p
 
-section EqvClosure
+section eqvClosure
 
 variable {T : Theory L} {C : Semiformula L ξ n → Prop}
 
@@ -153,151 +152,107 @@ lemma subset_equivalent_closure {p} : C p → EqvClosure T C p := by
   · rintro ⟨q, hq, hqp⟩
     exact ⟨q, ⟨q, hq, by rfl⟩, hqp⟩
 
-end EqvClosure
+end eqvClosure
 
-@[ext] structure Class (L : Language) where
-  Domain : {n : ℕ} → SyntacticSemiformula L n → Prop
-  rew_closed : ∀{n n'} (ω : Rew L ℕ n ℕ n'), ∀ p, Domain p → Domain (ω.hom p)
+abbrev UnitSemiformula (L : Language) (n : ℕ) := Semiformula L Unit n
+
+namespace Rew
+
+def unify : Rew L ξ n Unit n := Rew.rewriteMap (fun _ ↦ ())
+
+@[simp] lemma unify_bvar (x : Fin n) : unify (#x : Semiterm L ξ n) = #x := rfl
+
+@[simp] lemma unify_fvar (x : ξ) : unify (&x : Semiterm L ξ n) = &() := rfl
+
+@[simp] lemma q_unify : (unify : Rew L ξ n Unit n).q = unify := by ext x; { cases x using Fin.cases <;> simp }; { simp }
+
+end Rew
+
+@[ext] structure Class (L : Language) (ξ : Type*) where
+  Domain : {n : ℕ} → Semiformula L ξ n → Prop
+  rew_closed : ∀ {n n'}, ∀ ω : Rew L ξ n ξ n', ∀ p, Domain p → Domain (ω.hom p)
 
 namespace Class
 
-variable {c : Class L}
+variable {c : Class L ξ}
 
-protected def eqvClosure (c : Class L) (T : Theory L) : Class L where
-  Domain := EqvClosure T c.Domain
+/-
+lemma shift_closed {p : SyntacticFormula L} (hp : p ∈ c.Domain) : Rew.shift.hom p ∈ c.Domain := by
+  have : (Rew.hom (Rew.rewrite (&·.succ))) p ∈ c.Domain := c.rew_closed p hp (&·.succ)
+  have : @Rew.shift L 0 = Rew.rewrite (&·.succ) := by ext <;> simp
+  rw [this]; assumption
+-/
+
+protected def eqvClosure (c : Class L ξ) (T : Theory L) : Class L ξ where
+  Domain := fun {n} ↦ EqvClosure T c.Domain
   rew_closed := by
-    rintro _ _ ω p ⟨p', hp', H⟩;
+    rintro n n' ω p ⟨p', hp', H⟩
     exact ⟨ω.hom p', c.rew_closed ω p' hp', H.rew ω⟩
 
-def Mem (c : Class L) (p : Semiformula L ξ n) : Prop :=
-    ∃ f : ℕ → Semiterm L ξ n, ∃ p₀, c.Domain p₀ ∧ p = (Rew.rewrite f).hom p₀
-
-lemma mem_eqv_closure_Domain {p q : SyntacticSemiformula L n} (H : p ↔[T] q) : c.Domain p → (c.eqvClosure T).Domain q :=
-  fun hp ↦ ⟨p, hp, H⟩
-
-@[simp] lemma eqv_eqv : (c.eqvClosure T).eqvClosure T = c.eqvClosure T := by
-  ext; simp [Class.eqvClosure]
-
-lemma mem_eqv_closure_of_equiv_of_nonempty (hξ : Nonempty ξ) {p q : Semiformula L ξ n} (H : p ↔[T] q) : c.Mem p → (c.eqvClosure T).Mem q := by
-  haveI : Inhabited ξ := Classical.inhabited_of_nonempty hξ
-  rintro ⟨f, p, hp, rfl⟩
-  let q₀ : SyntacticSemiformula L n := (Rew.rewriteMap q.fvEnum).hom q
-  have hq : q = (Rew.rewriteMap q.fvEnumInv).hom q₀ := by simp [←Rew.hom_comp_app]
-  have hp' : Domain c (((Rew.rewriteMap q.fvEnum).comp (Rew.rewrite f)).hom p) :=
-    c.rew_closed ((Rew.rewriteMap q.fvEnum).comp (Rew.rewrite f)) p hp
-  have : Domain (c.eqvClosure T) q₀ :=
-    mem_eqv_closure_Domain (by simp [Rew.hom_comp_app]; exact H.rew _) hp'
-  exact ⟨_, q₀,this, hq⟩
-
-lemma mem_eqv_closure_of_equiv {p q : Semiformula L ξ n} (H : p ↔[T] q) : c.Mem p → (c.eqvClosure T).Mem q := by
-  by_cases hξ : Nonempty ξ
-  · exact mem_eqv_closure_of_equiv_of_nonempty hξ H
-  · haveI hξ : IsEmpty ξ := not_nonempty_iff.mp hξ
-    rintro ⟨f, p, hp, rfl⟩
-    let q₀ : SyntacticSemiformula L n := (Rew.rewriteMap hξ.elim).hom q
-    have hq : q = (Rew.rewrite (fun _ ↦ f 0)).hom q₀ := by
-      simp [←Rew.hom_comp_app]
-      symm; exact Rew.hom_eq_id_of_eq_on_fvar_list _ (fun x ↦ by simp [Rew.comp_app]) (fun x ↦ by simp)
-    have hp' : Domain c (((Rew.rewriteMap hξ.elim).comp (Rew.rewrite f)).hom p) :=
-    c.rew_closed ((Rew.rewriteMap hξ.elim).comp (Rew.rewrite f)) p hp
-    have : Domain (c.eqvClosure T) q₀ :=
-      mem_eqv_closure_Domain (by simp [Rew.hom_comp_app]; exact H.rew _) hp'
-    exact ⟨_, q₀,this, hq⟩
-
-lemma mem_of_equiv {p q : Semiformula L ξ n} (H : p ↔[T] q) : (c.eqvClosure T).Mem p → (c.eqvClosure T).Mem q := by
-  intro h; simpa using mem_eqv_closure_of_equiv H h
-
-lemma mem_iff_of_equiv {p q : Semiformula L ξ n} (H : p ↔[T] q) : (c.eqvClosure T).Mem p ↔ (c.eqvClosure T).Mem q :=
-  ⟨mem_of_equiv H, mem_of_equiv H.symm⟩
-
-lemma mem_of_domain {p : SyntacticSemiformula L n} (h : c.Domain p) : c.Mem p := ⟨(&·), _, h, by simp⟩
-
-lemma mem_rew {p₁ : Semiformula L ξ₁ n₁} (ω : Rew L ξ₁ n₁ ξ₂ n₂) : c.Mem p₁ → c.Mem (ω.hom p₁) := by
-  rintro ⟨f, p, hp, rfl⟩; simp [Mem]
-  let p' : SyntacticSemiformula L n₂ := (Rew.bind (fun x ↦ &↑x) (fun x ↦ &(x + n₁))).hom p
-  exact ⟨fun x ↦ if hx : x < n₁ then ω #⟨x, hx⟩ else ω (f (x - n₁)), p', c.rew_closed _ _ hp,
-    by simp [←Rew.hom_comp_app]; congr 2; ext <;> simp [Rew.comp_app]⟩
-
-lemma cast {p q : Semiformula L ξ n} (hp : c.Mem p) (e : p = q) : c.Mem q := e ▸ hp
-
-instance : LE (Class L) := ⟨fun c c' ↦ ∀ {n} {p : SyntacticSemiformula L n}, c.Domain p → c'.Domain p⟩
+instance : LE (Class L ξ) := ⟨fun c c' ↦ ∀ {n} {p : Semiformula L ξ n}, c.Domain p → c'.Domain p⟩
 
 namespace LE
 
-variable {c c' : Class L}
+variable {c c' : Class L ξ}
 
 @[refl] protected lemma refl : c ≤ c := id
 
-@[trans] protected lemma trans {c₁ c₂ c₃ : Class L} : c₁ ≤ c₂ → c₂ ≤ c₃ → c₁ ≤ c₃ := fun h₁ h₂ _ _ hp ↦ h₂ (h₁ hp)
-
-lemma Mem (H : c ≤ c') {p : Semiformula L ξ n} (hp : c.Mem p) : c'.Mem p := by
-  rcases hp with ⟨f, p, hp, rfl⟩
-  exact ⟨f, p, H hp, rfl⟩
+@[trans] protected lemma trans {c₁ c₂ c₃ : Class L ξ} : c₁ ≤ c₂ → c₂ ≤ c₃ → c₁ ≤ c₃ :=
+  fun h₁ h₂ _ _ hp ↦ h₂ (h₁ hp)
 
 end LE
 
-lemma le_eqvClosure (c : Class L) (T : Theory L) : c ≤ c.eqvClosure T := by intro _ p hp; exact subset_equivalent_closure hp
+lemma le_eqvClosure (c : Class L ξ) (T : Theory L) : c ≤ c.eqvClosure T := by intro _ p hp; exact subset_equivalent_closure hp
 
-lemma le_of_subtheory (c : Class L) {T T' : Theory L} (h : T ≾ T') : c.eqvClosure T ≤ c.eqvClosure T' := by
+lemma le_of_subtheory (c : Class L ξ) {T T' : Theory L} (h : T ≾ T') : c.eqvClosure T ≤ c.eqvClosure T' := by
   rintro _ p ⟨p', hp', H⟩; exact ⟨p', hp', H.of_subtheory h⟩
 
-class Atom (c : Class L) : Prop where
-  verum : ∀ n, c.Domain (⊤ : SyntacticSemiformula L n)
-  falsum : ∀ n, c.Domain (⊥ : SyntacticSemiformula L n)
-  rel : ∀ {n k} (r : L.Rel k) (v : Fin k → SyntacticSemiterm L n), c.Domain (Semiformula.rel r v)
-  nrel : ∀ {n k} (r : L.Rel k) (v : Fin k → SyntacticSemiterm L n), c.Domain (Semiformula.nrel r v)
+class Atom (c : Class L ξ) : Prop where
+  verum : ∀ n, c.Domain (⊤ : Semiformula L ξ n)
+  falsum : ∀ n, c.Domain (⊥ : Semiformula L ξ n)
+  rel : ∀ {n k} (r : L.Rel k) (v : Fin k → Semiterm L ξ n), c.Domain (Semiformula.rel r v)
+  nrel : ∀ {n k} (r : L.Rel k) (v : Fin k → Semiterm L ξ n), c.Domain (Semiformula.nrel r v)
 
-class Not (c : Class L) : Prop where
-  not {n} {p : SyntacticSemiformula L n} : c.Domain p → c.Domain (~p)
+class Not (c : Class L ξ) : Prop where
+  not {n} {p : Semiformula L ξ n} : c.Domain p → c.Domain (~p)
 
-class And (c : Class L) : Prop where
-  and {n} {p q : SyntacticSemiformula L n} : c.Domain p → c.Domain q → c.Domain (p ⋏ q)
+class And (c : Class L ξ) : Prop where
+  and {n} {p q : Semiformula L ξ n} : c.Domain p → c.Domain q → c.Domain (p ⋏ q)
 
-class Or (c : Class L) : Prop where
-  or {n} {p q : SyntacticSemiformula L n} : c.Domain p → c.Domain q → c.Domain (p ⋎ q)
+class Or (c : Class L ξ) : Prop where
+  or {n} {p q : Semiformula L ξ n} : c.Domain p → c.Domain q → c.Domain (p ⋎ q)
 
-class BAll (c : Class L) [L.LT] : Prop where
-  ball {n} {p : SyntacticSemiformula L (n + 1)} : c.Domain p → c.Domain (∀[“#0 < &0”] p)
+class BAll (c : Class L ξ) [L.LT] : Prop where
+  ball {n} {p : Semiformula L ξ (n + 1)} {t} : c.Domain p → t.Positive → c.Domain (∀[“#0 < !!t”] p)
 
-class BEx (c : Class L) [L.LT] : Prop where
-  bex {n} {p : SyntacticSemiformula L (n + 1)} : c.Domain p → c.Domain (∃[“#0 < &0”] p)
+class BEx (c : Class L ξ) [L.LT] : Prop where
+  bex {n} {p : Semiformula L ξ (n + 1)} {t} : c.Domain p → t.Positive → c.Domain (∃[“#0 < !!t”] p)
+
+class All (c : Class L ξ) [L.LT] : Prop where
+  all {n} {p : Semiformula L ξ (n + 1)} : c.Domain p → c.Domain (∀' p)
+
+class Ex (c : Class L ξ) [L.LT] : Prop where
+  ex {n} {p : Semiformula L ξ (n + 1)} : c.Domain p → c.Domain (∃' p)
 
 section Atom
 
 variable [c.Atom] [Nonempty (Term L ξ)]
 
-@[simp] lemma mem_verum : c.Mem (⊤ : Semiformula L ξ n) := by
-  let t : Semiterm L ξ n := Rew.substs ![] Classical.ofNonempty
-  simpa using mem_rew (Rew.bind ![] (fun _ ↦ t) : Rew L ℕ 0 ξ n) (mem_of_domain (Atom.verum _))
+attribute [simp] Atom.verum Atom.falsum Atom.rel Atom.nrel
 
-@[simp] lemma mem_falsum : c.Mem (⊥ : Semiformula L ξ n) := by
-  let t : Semiterm L ξ n := Rew.substs ![] Classical.ofNonempty
-  simpa using mem_rew (Rew.bind ![] (fun _ ↦ t) : Rew L ℕ 0 ξ n) (mem_of_domain (Atom.falsum _))
-
-@[simp] lemma mem_rel {k} (r : L.Rel k) (v : Fin k → Semiterm L ξ n) : c.Mem (Semiformula.rel r v) := by
-  let t : Semiterm L ξ n := Rew.substs ![] Classical.ofNonempty
-  have : c.Mem (Semiformula.rel (n := n) r (&↑·)) := (mem_of_domain (Atom.rel r (& ·)))
-  simpa [Rew.rel] using c.mem_rew (Rew.rewrite (fun x ↦ if hx : x < k then v ⟨x, hx⟩ else t) : Rew L ℕ n ξ n) this
-
-
-@[simp] lemma mem_nrel {k} (r : L.Rel k) (v : Fin k → Semiterm L ξ n) : c.Mem (Semiformula.nrel r v) := by
-  let t : Semiterm L ξ n := Rew.substs ![] Classical.ofNonempty
-  have : Mem c (Semiformula.nrel (n := n) r (&↑·)) := (mem_of_domain (Atom.nrel r (& ·)))
-  simpa [Rew.nrel] using mem_rew (Rew.rewrite (fun x ↦ if hx : x < k then v ⟨x, hx⟩ else t) : Rew L ℕ n ξ n) this
-
-@[simp] lemma mem_eq [L.Eq] (t u : Semiterm L ξ n) : c.Mem “!!t = !!u” := by
+@[simp] lemma mem_eq [L.Eq] (t u : Semiterm L ξ n) : c.Domain “!!t = !!u” := by
   simp [Semiformula.Operator.operator, Rew.rel, Semiformula.Operator.Eq.eq]
 
-@[simp] lemma mem_not_eq [L.Eq] (t u : Semiterm L ξ n) : c.Mem “!!t ≠ !!u” := by
+@[simp] lemma mem_not_eq [L.Eq] (t u : Semiterm L ξ n) : c.Domain “!!t ≠ !!u” := by
   simp [Semiformula.Operator.operator, Rew.rel, Semiformula.Operator.Eq.eq]
 
-@[simp] lemma mem_lt [L.LT] (t u : Semiterm L ξ n) : c.Mem “!!t < !!u” := by
+@[simp] lemma mem_lt [L.LT] (t u : Semiterm L ξ n) : c.Domain “!!t < !!u” := by
   simp [Semiformula.Operator.operator, Rew.rel, Semiformula.Operator.LT.lt]
 
-@[simp] lemma mem_not_lt [L.LT] (t u : Semiterm L ξ n) : c.Mem “!!t ≮ !!u” := by
+@[simp] lemma mem_not_lt [L.LT] (t u : Semiterm L ξ n) : c.Domain “!!t ≮ !!u” := by
   simp [Semiformula.Operator.operator, Rew.rel, Semiformula.Operator.LT.lt]
 
-def of_le (c c' : Class L) [c.Atom] (h : c ≤ c') : c'.Atom where
+def of_le (c c' : Class L ξ) [c.Atom] (h : c ≤ c') : c'.Atom where
   verum := fun n ↦ h (Atom.verum n)
   falsum := fun n ↦ h (Atom.falsum n)
   rel := fun r v ↦ h (Atom.rel r v)
@@ -311,10 +266,6 @@ section Not
 
 variable [c.Not]
 
-lemma mem_not {p : Semiformula L ξ n} (hp : c.Mem p) : c.Mem (~p) := by
-  rcases hp with ⟨f, p, hp, rfl⟩
-  simpa using mem_rew (Rew.rewrite f) (mem_of_domain (Not.not hp))
-
 instance : (c.eqvClosure T).Not := ⟨by rintro _ p ⟨p', hp', H⟩; exact ⟨~p', Not.not hp', H.not⟩⟩
 
 end Not
@@ -322,18 +273,6 @@ end Not
 section And
 
 variable [c.And]
-
-lemma mem_and {p q : Semiformula L ξ n} (hp : c.Mem p) (hq : c.Mem q) : c.Mem (p ⋏ q) := by
-  rcases hp with ⟨f, p, hp, rfl⟩
-  rcases hq with ⟨g, q, hq, rfl⟩
-  have hp' : c.Domain ((Rew.rewriteMap (Nat.bit false)).hom p) := c.rew_closed (Rew.rewriteMap (Nat.bit false)) _ hp
-  have hq' : c.Domain ((Rew.rewriteMap (Nat.bit true)).hom q) := c.rew_closed (Rew.rewriteMap (Nat.bit true)) _ hq
-  let fg : ℕ → Semiterm L ξ n :=
-    fun x ↦ Nat.bitCasesOn (C := fun _ ↦ Semiterm L ξ n) x (fun b x ↦ b.casesOn (f x) (g x))
-  refine cast (mem_rew (Rew.rewrite fg) <| c.mem_of_domain (And.and hp' hq')) ?_
-  simp [←Rew.hom_comp_app]; constructor
-  · congr; ext <;> simp [Rew.comp_app]
-  · congr; ext <;> simp [Rew.comp_app]
 
 instance : (c.eqvClosure T).And := ⟨by rintro _ p q ⟨p', hp', Hp⟩ ⟨q', hq', Hq⟩; exact ⟨p' ⋏ q', And.and hp' hq', Hp.and Hq⟩⟩
 
@@ -343,29 +282,17 @@ section Or
 
 variable [c.Or]
 
-lemma mem_or {p q : Semiformula L ξ n} (hp : c.Mem p) (hq : c.Mem q) : c.Mem (p ⋎ q) := by
-  rcases hp with ⟨f, p, hp, rfl⟩
-  rcases hq with ⟨g, q, hq, rfl⟩
-  have hp' : c.Domain ((Rew.rewriteMap (Nat.bit false)).hom p) := c.rew_closed _ _ hp
-  have hq' : c.Domain ((Rew.rewriteMap (Nat.bit true)).hom q) := c.rew_closed _ _ hq
-  let fg : ℕ → Semiterm L ξ n :=
-    fun x ↦ Nat.bitCasesOn (C := fun _ ↦ Semiterm L ξ n) x (fun b x ↦ b.casesOn (f x) (g x))
-  refine cast (mem_rew (Rew.rewrite fg) <| c.mem_of_domain (Or.or hp' hq')) ?_
-  simp [←Rew.hom_comp_app]; constructor
-  · congr; ext <;> simp [Rew.comp_app]
-  · congr; ext <;> simp [Rew.comp_app]
-
 instance : (c.eqvClosure T).Or := ⟨by rintro _ p q ⟨p', hp', Hp⟩ ⟨q', hq', Hq⟩; exact ⟨p' ⋎ q', Or.or hp' hq', Hp.or Hq⟩⟩
 
 variable [c.Not]
 
-lemma mem_imply {p q : Semiformula L ξ n} (hp : c.Mem p) (hq : c.Mem q) : c.Mem (p ⟶ q) := by
-  simp [Semiformula.imp_eq]; exact mem_or (mem_not hp) hq
+lemma mem_imply {p q : Semiformula L ξ n} (hp : c.Domain p) (hq : c.Domain q) : c.Domain (p ⟶ q) := by
+  simp [Semiformula.imp_eq]; exact Or.or (Not.not hp) hq
 
 variable [c.And]
 
-lemma mem_iff {p q : Semiformula L ξ n} (hp : c.Mem p) (hq : c.Mem q) : c.Mem (p ⟷ q) := by
-  simp [LO.LogicSymbol.iff]; exact mem_and (mem_imply hp hq) (mem_imply hq hp)
+lemma mem_iff {p q : Semiformula L ξ n} (hp : c.Domain p) (hq : c.Domain q) : c.Domain (p ⟷ q) := by
+  simp [LO.LogicSymbol.iff]; exact And.and (mem_imply hp hq) (mem_imply hq hp)
 
 end Or
 
@@ -373,32 +300,8 @@ section BAll
 
 variable [L.LT] [c.BAll]
 
-lemma mem_ball_aux (hξ : Nonempty ξ) {p : Semiformula L ξ (n + 1)} (hp : c.Mem p) {t : Semiterm L ξ (n + 1)} (ht : t.Positive) :
-    c.Mem (∀[“#0 < !!t”] p) := by
-  rcases hp with ⟨f, p, hp, rfl⟩
-  rcases Rew.positive_iff.mp ht with ⟨t, rfl⟩
-  haveI : Inhabited ξ := Classical.inhabited_of_nonempty hξ
-  generalize hp' : (Rew.rewrite f).hom p = p'
-  have : c.Mem (∀[“#0 < &0”] (Rew.rewrite (fun x ↦ &(p'.fvEnum x + 1))).hom p') :=
-    mem_of_domain <| BAll.ball (by simp [←hp', ←Rew.hom_comp_app]; exact c.rew_closed _ _ hp)
-  have : c.Mem (∀[“#0 < !!(Rew.bShift t)”] (Rew.rewriteMap $ p'.fvEnumInv ∘ p'.fvEnum).hom p') := by
-    simpa [-Rew.rewriteMap_fvEnumInv_fvEnum, Rew.rewriteMap, Function.comp,
-        ←Rew.hom_comp_app, Rew.rewrite_comp_rewrite, Function.comp] using
-      mem_rew (Rew.rewrite (t :>ₙ fun x ↦ &(p'.fvEnumInv x))) this
-  simpa using this
-
-lemma mem_ball {p : Semiformula L ξ (n + 1)} (hp : c.Mem p) {t : Semiterm L ξ (n + 1)} (ht : t.Positive) :
-    c.Mem (∀[“#0 < !!t”] p) := by
-  by_cases hξ : Nonempty ξ
-  · exact mem_ball_aux hξ hp ht
-  haveI : IsEmpty ξ := not_nonempty_iff.mp hξ
-  rcases hp with ⟨f, p, hp, rfl⟩
-  rcases Rew.positive_iff.mp ht with ⟨t, rfl⟩
-  generalize hp' : (Rew.rewrite f).hom p = p'
-  have : c.Mem (∀[“#0 < &0”] Rew.emb.hom p') :=
-    mem_of_domain <| BAll.ball (by simp [←hp', ←Rew.hom_comp_app]; exact c.rew_closed _ _ hp)
-  simpa [←Rew.hom_comp_app, Rew.rewrite_comp_rewrite, Function.comp] using
-    mem_rew (Rew.rewrite (fun _ ↦ t)) this
+instance : (c.eqvClosure T).BAll :=
+  ⟨by rintro n p t ⟨p', hp', H⟩ ht; exact ⟨∀[“#0 < !!t”] p', BAll.ball hp' ht, Semiformula.Equivalent.ball (by rfl) H⟩⟩
 
 end BAll
 
@@ -406,32 +309,8 @@ section BEx
 
 variable [L.LT] [c.BEx]
 
-lemma mem_bex_aux (hξ : Nonempty ξ) {p : Semiformula L ξ (n + 1)} (hp : c.Mem p) {t : Semiterm L ξ (n + 1)} (ht : t.Positive) :
-    c.Mem (∃[“#0 < !!t”] p) := by
-  rcases hp with ⟨f, p, hp, rfl⟩
-  rcases Rew.positive_iff.mp ht with ⟨t, rfl⟩
-  haveI : Inhabited ξ := Classical.inhabited_of_nonempty hξ
-  generalize hp' : (Rew.rewrite f).hom p = p'
-  have : c.Mem (∃[“#0 < &0”] (Rew.rewrite (fun x ↦ &(p'.fvEnum x + 1))).hom p') :=
-    mem_of_domain <| BEx.bex (by simp [←hp', ←Rew.hom_comp_app]; exact c.rew_closed _ _ hp)
-  have : c.Mem (∃[“#0 < !!(Rew.bShift t)”] (Rew.rewriteMap $ p'.fvEnumInv ∘ p'.fvEnum).hom p') := by
-    simpa [-Rew.rewriteMap_fvEnumInv_fvEnum, Rew.rewriteMap, Function.comp,
-        ←Rew.hom_comp_app, Rew.rewrite_comp_rewrite, Function.comp] using
-      mem_rew (Rew.rewrite (t :>ₙ fun x ↦ &(p'.fvEnumInv x))) this
-  simpa using this
-
-lemma mem_bex {p : Semiformula L ξ (n + 1)} (hp : c.Mem p) {t : Semiterm L ξ (n + 1)} (ht : t.Positive) :
-    c.Mem (∃[“#0 < !!t”] p) := by
-  by_cases hξ : Nonempty ξ
-  · exact mem_bex_aux hξ hp ht
-  haveI : IsEmpty ξ := not_nonempty_iff.mp hξ
-  rcases hp with ⟨f, p, hp, rfl⟩
-  rcases Rew.positive_iff.mp ht with ⟨t, rfl⟩
-  generalize hp' : (Rew.rewrite f).hom p = p'
-  have : c.Mem (∃[“#0 < &0”] Rew.emb.hom p') :=
-    mem_of_domain <| BEx.bex (by simp [←hp', ←Rew.hom_comp_app]; exact c.rew_closed _ _ hp)
-  simpa [←Rew.hom_comp_app, Rew.rewrite_comp_rewrite, Function.comp] using
-    mem_rew (Rew.rewrite (fun _ ↦ t)) this
+instance : (c.eqvClosure T).BEx :=
+  ⟨by rintro n p t ⟨p', hp', H⟩ ht; exact ⟨∃[“#0 < !!t”] p', BEx.bex hp' ht, Semiformula.Equivalent.bex (by rfl) H⟩⟩
 
 end BEx
 
@@ -439,35 +318,35 @@ section
 
 variable [c.Atom] [c.And] [c.Or] [Nonempty (Term L ξ)]
 
-@[simp] lemma mem_le [L.Eq] [L.LT] (t u : Semiterm L ξ n) : c.Mem “!!t ≤ !!u” := by
+@[simp] lemma mem_le [L.Eq] [L.LT] (t u : Semiterm L ξ n) : c.Domain “!!t ≤ !!u” := by
   simp [Semiformula.Operator.operator, Rew.rel,
     Semiformula.Operator.LE.sentence_eq, Semiformula.Operator.Eq.eq, Semiformula.Operator.LT.lt]
-  apply mem_or <;> simp
+  apply Or.or <;> simp
 
-@[simp] lemma mem_not_le [L.Eq] [L.LT] (t u : Semiterm L ξ n) : c.Mem “¬!!t ≤ !!u” := by
+@[simp] lemma mem_not_le [L.Eq] [L.LT] (t u : Semiterm L ξ n) : c.Domain “¬!!t ≤ !!u” := by
   simp [Semiformula.Operator.operator, Rew.rel,
     Semiformula.Operator.LE.sentence_eq, Semiformula.Operator.Eq.eq, Semiformula.Operator.LT.lt]
-  apply mem_and <;> simp
+  apply And.and <;> simp
 
 end
 
 end Class
 
-def openClass (L : Language) : Class L where
+def openClass (L : Language) (ξ : Type*) : Class L ξ where
   Domain := Semiformula.Open
   rew_closed := by simp
 
-instance : (openClass L).Atom where
+instance : (openClass L ξ).Atom where
   verum := fun _ ↦ Semiformula.open_top
   falsum := fun _ ↦ Semiformula.open_bot
   rel := fun r v ↦ Semiformula.open_rel r v
   nrel := fun r v ↦ Semiformula.open_nrel r v
 
-instance : (openClass T).Not := ⟨Semiformula.open_neg.mpr⟩
+instance : (openClass T ξ).Not := ⟨Semiformula.open_neg.mpr⟩
 
-instance : (openClass T).And := ⟨fun hp hq ↦ Semiformula.open_and.mpr ⟨hp, hq⟩⟩
+instance : (openClass T ξ).And := ⟨fun hp hq ↦ Semiformula.open_and.mpr ⟨hp, hq⟩⟩
 
-instance : (openClass T).Or := ⟨fun hp hq ↦ Semiformula.open_or.mpr ⟨hp, hq⟩⟩
+instance : (openClass T ξ).Or := ⟨fun hp hq ↦ Semiformula.open_or.mpr ⟨hp, hq⟩⟩
 
 section
 
@@ -477,17 +356,22 @@ open Lean.Parser.Tactic (config)
 attribute [aesop 1 (rule_sets [FormulaClass]) norm]
   Class.mem_imply
   Class.mem_iff
-  Class.mem_ball
-  Class.mem_bex
 
-attribute [aesop 2 (rule_sets [FormulaClass]) norm]
-  Class.mem_and
-  Class.mem_or
-  Class.mem_rew
-  Class.mem_not
+attribute [aesop 3 (rule_sets [FormulaClass]) norm]
+  Class.BAll.ball
+  Class.BEx.bex
+
+attribute [aesop 3 (rule_sets [FormulaClass]) norm]
+  Class.And.and
+  Class.Or.or
+  Class.rew_closed
+  Class.Not.not
+  Class.All.all
+  Class.Ex.ex
+
 
 macro "formula_class" : attr =>
-  `(attr|aesop 4 (rule_sets [$(Lean.mkIdent `FormulaClass):ident]) safe)
+  `(attr|aesop 0 (rule_sets [$(Lean.mkIdent `FormulaClass):ident]) safe)
 
 macro "formula_class" (config)? : tactic =>
   `(tactic| aesop (options := { terminal := true }) (rule_sets [$(Lean.mkIdent `FormulaClass):ident]))
@@ -495,7 +379,7 @@ macro "formula_class" (config)? : tactic =>
 macro "formula_class?" (config)? : tactic =>
   `(tactic| aesop? (options := { terminal := true }) (rule_sets [$(Lean.mkIdent `FormulaClass):ident]))
 
-example : (openClass ℒₒᵣ).Mem (“¬0 < 6 → &6 + #5 ≠ 0” : Semiformula ℒₒᵣ ℕ 8) := by { formula_class }
+example : (openClass ℒₒᵣ ℕ).Domain (“¬0 < 6 → &6 + #5 ≠ 0” : Semiformula ℒₒᵣ ℕ 8) := by { formula_class }
 
 end
 
